x86/TranslateInstrSize.v
@@ -10,25 +10,6 @@ Local Open Scope error_monad_scope.
 Local Open Scope hex_scope.
 Local Open Scope bits_scope.
 
-(* TODO *)
-Definition Instr_size_aux (i: Instruction) :=
-  1.
-
-Definition Instr_size (l : list Instruction) :=
-  match l with
-  | Override :: REX_WRXB w r x b :: i :: tl
-  | REP :: REX_WRXB w r x b :: i :: tl
-  | REPNZ :: REX_WRXB w r x b :: i :: tl =>
-    2 + Instr_size_aux i
-  | REX_WRXB _ _ _ _ :: i :: tl
-  | Override :: i :: tl
-  | REP :: i :: tl 
-  | REPNZ :: i :: tl =>
-    1 + Instr_size_aux i
-  | i :: tl =>
-    Instr_size_aux i
-  | _ => 0
-  end.
 
 Lemma instr_eq_size: forall i1 i2,
     instr_eq i1 i2 -> instr_size_asm i1 = instr_size_asm i2.
@@ -43,18 +24,19 @@ Proof.
   admit.
 
   unfold rex_prefix_check_rr,rex_prefix_check_r.
-  rewrite PTR. auto.
+  rewrite PTR. destr.
+  apply andb_true_iff in Heqb. destruct Heqb.
+  rewrite H. auto.
+  apply andb_false_iff in Heqb. destruct Heqb.
+  rewrite H. auto.
+  rewrite H. auto.
 
+  destruct H11. subst. auto.
+  
   -
     destruct i1;try inv H;destruct i2;try inv H;cbn [instr_size_asm];auto.
     
 Admitted.
 
-
-Lemma translate_instr_size: forall i e l l',
-      translate_instr e i = OK l ->
-      Instr_size (l ++ l') = instr_size_asm i.
-Proof.
-Admitted.
 
 
